Revert "Add list"
This reverts commit 2036bbf6d6ce1ee51ba22e7d0af4ef2f313d85d7.

TestModels/Aggregate/src/SimpleAggregateImpl.dfy
@@ -12,8 +12,19 @@ module SimpleAggregateImpl refines AbstractSimpleAggregateOperations {
     predicate GetAggregateEnsuresPublicly(input: GetAggregateInput, output: Result<GetAggregateOutput, Error>) {
         true
     }
+    predicate GetAggregateKnownValueTestEnsuresPublicly(input: GetAggregateInput, output: Result<GetAggregateOutput, Error>) {
+        true
+    }
     method GetAggregate(config: InternalConfig, input: GetAggregateInput )
     returns (output: Result<GetAggregateOutput, Error>) {
+        var res := GetAggregateOutput(recursiveUnion := input.recursiveUnion);
+        return Success(res);
+    }
+
+    // This method is only used for known-value testing. See "Known Value Tests" inside TestModels' README file.
+    method GetAggregateKnownValueTest(config: InternalConfig, input: GetAggregateInput )
+    returns (output: Result<GetAggregateOutput, Error>) {
+        ValidateInput(input);
         var res := GetAggregateOutput(recursiveUnion := input.recursiveUnion);
         return Success(res);
     }
