TestModels/Aggregate/test/SimpleAggregateImplTest.dfy
@@ -19,16 +19,30 @@ module SimpleAggregateImplTest {
         var myDataMap: StructuredDataMap := map[];
         // myDataMap := myDataMap["key1" := StructuredData(content := Some(42))];
         myDataMap := myDataMap["key2" := StructuredData(content := Some(IntegerValue(42)))];
-        var myList: ListWithRecursion := [myDataMap];
-        var recursiveUnion := ListValue(myList);
+        var recursiveUnion := DataMap(myDataMap);
 
         var ret :- expect client.GetAggregate(GetAggregateInput(
                                                                 recursiveUnion := Some(recursiveUnion)
                                                                 ));
         expect ret.recursiveUnion.Some?;
-        expect ret.recursiveUnion.value.ListValue?;
-        expect ret.recursiveUnion.value.ListValue == myList;
+        expect ret.recursiveUnion.value.DataMap?;
+        expect ret.recursiveUnion.value.DataMap == myDataMap;
 
         print ret;
     }
+
+    method TestGetAggregateKnownValue(client: ISimpleAggregateClient)
+    requires client.ValidState()
+      modifies client.Modifies
+      ensures client.ValidState()
+      {
+        var myDataMap: StructuredDataMap := map[];
+        // myDataMap := myDataMap["key1" := StructuredData(content := Some(42))];
+        myDataMap := myDataMap["key2" := StructuredData(content := Some(IntegerValue(42)))];
+        var recursiveUnion := DataMap(myDataMap);
+        var ret :- expect client.GetAggregate(GetAggregateInput(recursiveUnion := Some(recursiveUnion)));
+        expect ret.recursiveUnion.Some?;
+        expect ret.recursiveUnion.value.DataMap?;
+        expect ret.recursiveUnion.value.DataMap == myDataMap;    
+      }
 }
